hw6 left with one error

Assignment 6/Homework6.dfy
@@ -5,7 +5,7 @@ function flatten<T>(tree:Tree<T>):List<T>
 {
     match tree
     case Leaf => Nil
-    case Node(leftTree, rightTree, x) => Cons(x, append(flatten(leftTree), flatten(rightTree)))
+    case Node(leftTree, rightTree, x) => append(flatten(leftTree), Cons(x, flatten(rightTree)))
 }
 
 function append<T>(xs:List<T>, ys:List<T>):List<T>
@@ -34,10 +34,23 @@ lemma sameElements<T>(tree:Tree<T>, element:T)
 ensures treeContains(tree, element) <==> listContains(flatten(tree), element)
 {
 	match tree
-        case Leaf => {}
-        case Node(leftTree, rightTree, x) => 
-        {
-            sameElements(leftTree, element)
-            sameElements(rightTree, element)
-        }
+    case Leaf => {}
+    case Node(leftTree, rightTree, x) => {
+        sameElements(leftTree, x);
+        sameElements(rightTree, x);
+
+        assert treeContains(tree, element)
+            == (treeContains(leftTree, element) || treeContains(rightTree, element) || x == element)
+            == (listContains(flatten(leftTree), element) || listContains(flatten(rightTree), element) || x == element)
+            == (listContains(flatten(leftTree), element) || (listContains(Cons(x, flatten(rightTree)), element)))
+            == listContains(append(flatten(leftTree), Cons(x, flatten(rightTree))), element)
+            == listContains(flatten(tree), element);
+    
+        assert listContains(flatten(tree), element)
+            == listContains(append(flatten(leftTree), Cons(x, flatten(rightTree))), element)
+            == (listContains(flatten(leftTree), element) || listContains(Cons(x, flatten(rightTree)), element))
+            == (listContains(flatten(leftTree), element) || listContains(flatten(rightTree), element) || x == element)
+            == (treeContains(leftTree, element) || treeContains(rightTree, element) || x == element)
+            == treeContains(tree, element);
+    }
 }
